Refactor parser combinators

src/ConcreteMath/ParserCombinators.thy
@@ -4,38 +4,38 @@ theory ParserCombinators
     Main
     Show.Show
     "HOL-Library.Monad_Syntax"
-    Certification_Monads.Error_Monad
+    "HOL-Library.Sublist"
 begin
 
 type_synonym error_message_type = string
 
-type_synonym ('i, 'o) parser_scheme = "'i list \<Rightarrow> error_message_type + ('i list \<times> 'o)"
+type_synonym ('i, 'o) parser_function = "'i list \<Rightarrow> error_message_type + ('i list \<times> 'o)"
 
-definition is_parser :: "('i, 'o) parser_scheme \<Rightarrow> bool" where
-  "is_parser p \<equiv> \<forall>i r v. p i = return (r, v) \<longrightarrow> length i \<ge> length r"
+definition is_parser :: "('i, 'o) parser_function \<Rightarrow> bool" where
+  "is_parser p \<equiv> \<forall>i r v. p i = Inr (r, v) \<longrightarrow> length i \<ge> length r"
 
 lemma is_parserI [intro]:
-  assumes "\<And>i r v. p i = return (r, v) \<Longrightarrow> length i \<ge> length r"
+  assumes "\<And>i r v. p i = Inr (r, v) \<Longrightarrow> length i \<ge> length r"
   shows "is_parser p"
   using assms is_parser_def by blast
 
 lemma is_parserE [elim]:
   assumes "is_parser p"
-    and "(\<And>i r v. p i = return (r, v) \<Longrightarrow> length i \<ge> length r) \<Longrightarrow> P"
+    and "(\<And>i r v. p i = Inr (r, v) \<Longrightarrow> length i \<ge> length r) \<Longrightarrow> P"
   shows "P"
   using assms by (simp add: is_parser_def)
 
-definition greedy_parser :: "('i, 'o) parser_scheme \<Rightarrow> bool" where
-  "greedy_parser p \<equiv> \<forall>i r v. p i = return (r, v) \<longrightarrow> length i > length r"
+definition greedy_parser :: "('i, 'o) parser_function \<Rightarrow> bool" where
+  "greedy_parser p \<equiv> \<forall>i r v. p i = Inr (r, v) \<longrightarrow> length i > length r"
 
 lemma greedy_parserI [intro]:
-  assumes "\<And>i r v. p i = return (r, v) \<Longrightarrow> length i > length r"
+  assumes "\<And>i r v. p i = Inr (r, v) \<Longrightarrow> length i > length r"
   shows "greedy_parser p"
   using assms greedy_parser_def by blast
 
 lemma greedy_parserE [elim]:
   assumes "greedy_parser p"
-    and "(\<And>i r v. p i = return (r, v) \<Longrightarrow> length i > length r) \<Longrightarrow> P"
+    and "(\<And>i r v. p i = Inr (r, v) \<Longrightarrow> length i > length r) \<Longrightarrow> P"
   shows "P"
   using assms by (simp add: greedy_parser_def)
 
@@ -44,68 +44,295 @@ lemma greedy_parser_implies_is_parser:
   unfolding is_parser_def greedy_parser_def
   by (simp add: nat_less_le)
 
-typedef ('i, 'o) greedy_parser_scheme = "{p::('i, 'o) parser_scheme. (greedy_parser p)}"
-morphisms rep_greedy abs_greedy
-by auto
+typedef ('i, 'o) parser_scheme = "{p::('i, 'o) parser_function. is_parser p}"
+morphisms run_parser abs_parser by auto
+setup_lifting type_definition_parser_scheme
 
+typedef ('i, 'o) greedy_parser_scheme = "{p::('i, 'o) parser_function. greedy_parser p}"
+morphisms run_greedy abs_greedy by auto
 setup_lifting type_definition_greedy_parser_scheme
-
-definition expected :: "string \<Rightarrow> ('t::show, 'a) parser_scheme" where
-  "expected msg ts = error
-    (''Expected '' @ msg @ '', but found: '' @ shows_quote (shows (take 30 ts)) [])"
 
 subsection \<open>Primitive Combinators\<close>
 
+subsubsection \<open>Fail\<close>
 definition
-  fail :: "error_message_type \<Rightarrow> ('i, 'o) parser_scheme" where
-  "fail msg i = error msg"
+  fail_raw :: "error_message_type \<Rightarrow> ('i, 'o) parser_function" where
+  "fail_raw msg i = Inl msg"
 
-definition
-  pure :: "'o \<Rightarrow> ('i, 'o) parser_scheme" where
-  "pure output i = return (i, output)"
+lemma fail_is_greedy_parser [intro]:
+  "greedy_parser (fail_raw s)"
+  by (simp add: fail_raw_def greedy_parser_def)
 
-(* TODO: Add show*)
+lemma fail_is_parser [intro]:
+  "is_parser (fail_raw s)"
+  using greedy_parser_implies_is_parser by blast
+
+lift_definition
+  fail :: "error_message_type \<Rightarrow> ('i, 'o) parser_scheme"
+  is fail_raw by blast
+
+lift_definition
+  fail\<g> :: "error_message_type \<Rightarrow> ('i, 'o) greedy_parser_scheme"
+  is fail_raw by blast
+
+subsubsection \<open>Expected\<close>
 definition
-  satisfy :: "('i \<Rightarrow> bool) \<Rightarrow> ('i::show, 'i) parser_scheme" where
-  "satisfy P xs =
+  expected_raw :: "string \<Rightarrow> ('t::show, 'a) parser_function" where
+  "expected_raw msg ts = Inl
+    (''Expected '' @ msg @ '', but found: '' @ shows_quote (shows (take 30 ts)) [])"
+
+lemma expected_raw_is_parser [intro]:
+  "is_parser (expected_raw s)"
+  unfolding is_parser_def expected_raw_def shows_quote_def
+  by fastforce
+
+lemma expected_raw_is_greedy_parser [intro]:
+  "greedy_parser (expected_raw s)"
+  unfolding greedy_parser_def expected_raw_def shows_quote_def
+  by fastforce
+
+lift_definition
+  expected :: "string \<Rightarrow> ('t::show, 'a) parser_scheme"
+  is expected_raw by blast
+
+lift_definition
+  expected\<g> :: "string \<Rightarrow> ('t::show, 'a) greedy_parser_scheme"
+  is expected_raw by blast
+
+subsubsection \<open>Pure\<close>
+definition
+  pure_raw :: "'o \<Rightarrow> ('i, 'o) parser_function" where
+  "pure_raw output i = Inr (i, output)"
+
+lemma pure_raw_is_parser [intro]:
+  "is_parser (pure_raw x)"
+  by (simp add: is_parser_def pure_raw_def)
+
+lift_definition
+  pure :: "'o \<Rightarrow> ('i, 'o) parser_scheme"
+  is pure_raw by blast
+
+subsubsection \<open>Satisfy\<close>
+definition
+  satisfy_raw :: "('i \<Rightarrow> bool) \<Rightarrow> ('i::show, 'i) parser_function" where
+  "satisfy_raw P xs =
     (case xs of
-       []   \<Rightarrow> expected ''symbol that satisfies predicate'' xs
-     | x#xs \<Rightarrow> if P x then Inr (xs, x) else error ''hi'')"
+       []   \<Rightarrow> expected_raw ''symbol that satisfies predicate'' xs
+     | x#xs \<Rightarrow> if P x then Inr (xs, x) else Inl ''satisfy predicate failed'')"
 
+lemma satisfy_is_greedy_parser [intro]:
+  "greedy_parser (satisfy_raw P)"
+  unfolding greedy_parser_def satisfy_raw_def expected_def expected_raw_def
+  using expected_raw_is_parser
+    by (simp add: list.case_eq_if)
+
+lift_definition
+  satisfy\<g> :: "('i \<Rightarrow> bool) \<Rightarrow> ('i::show, 'i) greedy_parser_scheme"
+  is satisfy_raw by blast
+
+subsubsection \<open>Bind\<close>
 definition
-  bind :: "('i, 'a) parser_scheme \<Rightarrow> ('a \<Rightarrow> ('i, 'b) parser_scheme) \<Rightarrow> ('i, 'b) parser_scheme" where
-  "bind p k i =
+  bind_raw :: "('i, 'a) parser_function \<Rightarrow> ('a \<Rightarrow> ('i, 'b) parser_function) \<Rightarrow> ('i, 'b) parser_function" where
+  "bind_raw p k i =
     (case p i of
        Inl err \<Rightarrow> Inl err
      | Inr (rest, output) \<Rightarrow> k output rest)"
 
+(* NOTE: Following four lemmas Look like `\<or>` truth table, could this be simplified? *)
+lemma bind_raw_is_parser [intro]:
+  assumes "is_parser p" and "\<And>x. is_parser (f x)" shows "is_parser (bind_raw p f)"
+  unfolding greedy_parser_def bind_raw_def is_parser_def
+  by (smt (verit, ccfv_SIG) Inl_Inr_False assms is_parser_def order_trans prod.split_sel split_beta sum.case_eq_if sum.collapse(2) sum.disc(2))
+
+lift_definition
+  bind :: "('i, 'a) parser_scheme \<Rightarrow> ('a \<Rightarrow> ('i, 'b) parser_scheme) \<Rightarrow> ('i, 'b) parser_scheme"
+  is bind_raw by auto
+
+lemma bind_raw_is_greedy_parser [intro]:
+  assumes "greedy_parser p" and "\<And>x. greedy_parser (f x)" shows "greedy_parser (bind_raw p f)"
+  unfolding greedy_parser_def
+  by (smt (verit) Inl_Inr_False ParserCombinators.bind_raw_def assms greedy_parserE order_less_trans prod.split_sel split_beta sum.case_eq_if sum.collapse(2) sum.disc(2))
+
+lift_definition
+  bind\<g> :: "('i, 'a) greedy_parser_scheme \<Rightarrow> ('a \<Rightarrow> ('i, 'b) greedy_parser_scheme) \<Rightarrow> ('i, 'b) greedy_parser_scheme"
+  is bind_raw by blast
+
+lemma greedy_parser_bind_raw_is_greedy_parser [intro]:
+  assumes "greedy_parser p" and "\<And>x. is_parser (f x)" shows "greedy_parser (bind_raw p f)"
+  unfolding greedy_parser_def bind_raw_def
+  by (smt (verit, ccfv_SIG) Inl_Inr_False assms dual_order.strict_trans2 greedy_parser_def is_parserE prod.split_sel split_beta sum.case_eq_if sum.collapse(2) sum.disc(2))
+
+lift_definition
+  bind\<g>\<l> :: "('i, 'a) greedy_parser_scheme \<Rightarrow> ('a \<Rightarrow> ('i, 'b) parser_scheme) \<Rightarrow> ('i, 'b) greedy_parser_scheme"
+  is bind_raw by blast
+
+lemma parser_greedy_bind_raw_is_greedy_parser [intro]:
+  assumes "is_parser p" and "\<And>x. greedy_parser (f x)" shows "greedy_parser (bind_raw p f)"
+  unfolding greedy_parser_def bind_raw_def
+  by (smt (verit, best) Inl_Inr_False assms greedy_parserE is_parserE linorder_not_less not_less_iff_gr_or_eq order_less_trans prod.split_sel split_beta sum.case_eq_if sum.collapse(2) sum.disc(2))
+
+lift_definition
+  bind\<g>\<r> :: "('i, 'a) parser_scheme \<Rightarrow> ('a \<Rightarrow> ('i, 'b) greedy_parser_scheme) \<Rightarrow> ('i, 'b) greedy_parser_scheme"
+  is bind_raw by (simp add: parser_greedy_bind_raw_is_greedy_parser)
+
 adhoc_overloading
-  Monad_Syntax.bind bind
+  Monad_Syntax.bind bind_raw bind bind\<g> bind\<g>\<l> bind\<g>\<r>
 
+subsubsection \<open>Map\<close>
 definition
-  map :: "('a \<Rightarrow> 'b) \<Rightarrow> ('i, 'a) parser_scheme \<Rightarrow> ('i, 'b) parser_scheme" (infixl "<$>" 58) where
-  "map f p i =
-    (case p i of
-       Inl err \<Rightarrow> Inl err
-     | Inr (i', v) \<Rightarrow> Inr (i', f v))"
+  map_raw :: "('a \<Rightarrow> 'b) \<Rightarrow> ('i, 'a) parser_function \<Rightarrow> ('i, 'b) parser_function" (infixl "<$>\<r>" 58) where
+  "map_raw f p  = do {
+    x \<leftarrow> p;
+    pure_raw (f x)
+  }"
 
-definition
-  product :: "('i, 'a) parser_scheme \<Rightarrow> ('i, 'b) parser_scheme \<Rightarrow> ('i, 'a \<times> 'b) parser_scheme" where
-  "product p1 p2 i =
-    (case p1 i of
-       Inl err \<Rightarrow> Inl err
-     | Inr (i1, v1) \<Rightarrow>
-       (case p2 i1 of
-          Inl err' \<Rightarrow> Inl err'
-        | Inr (i2, v2) \<Rightarrow> Inr (i2, (v1, v2))))"
+lemma map_raw_is_parser [intro]:
+  assumes "is_parser p" shows "is_parser (map_raw f p)"
+  by (simp add: assms bind_raw_is_parser map_raw_def pure_raw_is_parser)
 
+lift_definition
+  map :: "('a \<Rightarrow> 'b) \<Rightarrow> ('i, 'a) parser_scheme \<Rightarrow> ('i, 'b) parser_scheme" (infixl "<$>" 58)
+  is map_raw by blast
+
+lemma map_raw_is_greedy_parser [intro]:
+  assumes "greedy_parser p" shows "greedy_parser (map_raw f p)"
+  by (simp add: assms greedy_parser_bind_raw_is_greedy_parser map_raw_def pure_raw_is_parser)
+
+lift_definition
+  mapG :: "('a \<Rightarrow> 'b) \<Rightarrow> ('i, 'a) greedy_parser_scheme \<Rightarrow> ('i, 'b) greedy_parser_scheme" (infixl "<$>\<g>" 58)
+  is map_raw by blast
+
+subsubsection \<open>Product\<close>
+(* TODO: Rewrite with overloaded definition *)
 definition
-  either :: "('i, 'a) parser_scheme \<Rightarrow> ('i, 'a) parser_scheme \<Rightarrow> ('i, 'a) parser_scheme" (infixl "<|>" 57)
+  product_raw :: "('i, 'a) parser_function \<Rightarrow> ('i, 'b) parser_function \<Rightarrow> ('i, 'a \<times> 'b) parser_function" where
+  "product_raw p q = do {
+    a \<leftarrow> p;
+    b \<leftarrow> q;
+    pure_raw (a, b)
+  }"
+
+(* NOTE: Following four lemmas Look like `\<or>` truth table, could this be simplified? *)
+lemma product_raw_is_parser [intro]:
+  assumes "is_parser p" and "is_parser q" shows "is_parser (product_raw p q)"
+  unfolding product_raw_def
+  by (simp add: assms bind_raw_is_parser pure_raw_is_parser)
+
+lift_definition
+  product :: "('i, 'a) parser_scheme \<Rightarrow> ('i, 'b) parser_scheme \<Rightarrow> ('i, 'a \<times> 'b) parser_scheme"
+  is product_raw by blast
+
+lemma product_raw_is_greedy_parser [intro]:
+  assumes "greedy_parser p" and "greedy_parser q" shows "greedy_parser (product_raw p q)"
+  unfolding product_raw_def
+  by (simp add: assms greedy_parser_bind_raw_is_greedy_parser greedy_parser_implies_is_parser pure_raw_is_parser)
+
+lift_definition
+  product\<g> :: "('i, 'a) greedy_parser_scheme \<Rightarrow> ('i, 'b) greedy_parser_scheme \<Rightarrow> ('i, 'a \<times> 'b) greedy_parser_scheme"
+  is product_raw by blast
+
+lemma parser_greedy_product_raw_is_greedy_parser [intro]:
+  assumes "is_parser p" and "greedy_parser q" shows "greedy_parser (product_raw p q)"
+  by (simp add: assms(1) assms(2) greedy_parser_bind_raw_is_greedy_parser parser_greedy_bind_raw_is_greedy_parser product_raw_def pure_raw_is_parser)
+
+lift_definition
+  product\<g>\<r> :: "('i, 'a) parser_scheme \<Rightarrow> ('i, 'b) greedy_parser_scheme \<Rightarrow> ('i, 'a \<times> 'b) greedy_parser_scheme"
+  is product_raw by blast
+
+lemma greedy_parser_product_raw_is_greedy_parser [intro]:
+  assumes "greedy_parser p" and "is_parser q" shows "greedy_parser (product_raw p q)"
+  unfolding product_raw_def
+  by (simp add: assms bind_raw_is_parser greedy_parser_bind_raw_is_greedy_parser pure_raw_is_parser)
+
+lift_definition
+  product\<g>\<l> :: "('i, 'a) greedy_parser_scheme \<Rightarrow> ('i, 'b) parser_scheme \<Rightarrow> ('i, 'a \<times> 'b) greedy_parser_scheme"
+  is product_raw by blast
+
+subsubsection \<open>Either\<close>
+definition
+  either_raw :: "('i, 'a) parser_function \<Rightarrow> ('i, 'a) parser_function \<Rightarrow> ('i, 'a) parser_function" (infixl "<|>\<r>" 57)
 where
-  "either p1 p2 i =
+  "either_raw p1 p2 i =
     (case p1 i of
       Inr output \<Rightarrow> Inr output
     | Inl _ \<Rightarrow> p2 i)"
+
+lemma alternative_indepotent[simp]:
+  "(u <|>\<r> u) = u"
+proof -
+  have "\<And>i. (u <|>\<r> u) i = u i" by (simp add: either_raw_def sum.case_eq_if)
+  thus ?thesis by auto
+qed
+
+lemma alternative_associativity:
+  "(u <|>\<r> (v <|>\<r> w)) = ((u <|>\<r> v) <|>\<r> w)"
+  unfolding either_raw_def
+  by (auto split: sum.split)
+
+lemma either_raw_parsers:
+  assumes "is_parser (either_raw p q)" shows "is_parser p \<or> is_parser q"
+  unfolding either_raw_def is_parser_def
+  by (metis assms either_raw_def is_parser_def sum.case(2))
+
+lemma either_raw_greedy_parsers:
+  assumes "greedy_parser (either_raw p q)" shows "greedy_parser p \<or> greedy_parser q"
+  unfolding either_raw_def greedy_parser_def
+  by (metis assms either_raw_def greedy_parser_def sum.case(2))
+
+lemma either_raw_is_parser [intro]:
+  assumes "is_parser p" and "is_parser q" shows "is_parser (either_raw p q)"
+  unfolding either_raw_def
+  by (smt (verit) assms is_parser_def sum.case_eq_if sum.disc(2) sum.expand sum.sel(2))
+
+lift_definition
+  either :: "('i, 'a) parser_scheme \<Rightarrow> ('i, 'a) parser_scheme \<Rightarrow> ('i, 'a) parser_scheme" (infixl "<|>" 57)
+  is either_raw by blast
+
+lemma either_raw_is_greedy_parser [intro]:
+  assumes "greedy_parser p" and "greedy_parser q" shows "greedy_parser (either_raw p q)"
+  unfolding either_raw_def
+  by (metis (mono_tags, lifting) assms greedy_parser_def sum.case_eq_if sum.collapse(2))
+
+lift_definition
+  either\<g> :: "('i, 'a) greedy_parser_scheme \<Rightarrow> ('i, 'a) greedy_parser_scheme \<Rightarrow> ('i, 'a) greedy_parser_scheme" (infixl "<|>\<g>" 57)
+  is either_raw by blast
+
+lemma parser_greedy_either_raw_is_parser [intro]:
+  assumes "is_parser p" and "greedy_parser q" shows "is_parser (either_raw p q)"
+  unfolding either_raw_def is_parser_def
+  by (metis assms greedy_parserE is_parserE less_imp_le_nat sum.case_eq_if sum.collapse(2))
+
+lift_definition
+  either\<p>\<l> :: "('i, 'a) parser_scheme \<Rightarrow> ('i, 'a) greedy_parser_scheme \<Rightarrow> ('i, 'a) parser_scheme" (infixl "<|>\<p>\<l>" 57)
+  is either_raw by blast
+
+lemma greedy_parser_either_raw_is_parser [intro]:
+  assumes "greedy_parser p" and "is_parser q" shows "is_parser (either_raw p q)"
+  unfolding either_raw_def is_parser_def greedy_parser_def
+  by (metis assms greedy_parser_implies_is_parser is_parserE sum.case_eq_if sum.collapse(2))
+
+lift_definition
+  either\<p>\<r> :: "('i, 'a) greedy_parser_scheme \<Rightarrow> ('i, 'a) parser_scheme \<Rightarrow> ('i, 'a) parser_scheme" (infixl "<|>\<p>\<r>" 57)
+  is either_raw by blast
+
+lemma greedy_parser_either_raw_fail [simp]:
+  "greedy_parser (p <|>\<r> fail_raw s) = greedy_parser p"
+  unfolding fail_raw_def
+  by (metis Inl_Inr_False either_raw_def either_raw_is_greedy_parser greedy_parser_def sum.case(2))
+
+lemma greedy_parser_either_raw_expected [simp]:
+  "greedy_parser (p <|>\<r> expected_raw s) = greedy_parser p"
+  unfolding expected_raw_def
+  by (smt (verit, best) Inl_Inr_False either_raw_def either_raw_is_greedy_parser greedy_parser_def sum.case(2))
+
+lemma is_parser_either_raw_fail [simp]:
+  "is_parser (p <|>\<r> fail_raw s) = is_parser p"
+  by (metis (full_types) either_raw_def either_raw_is_parser fail_is_parser is_parser_def old.sum.simps(6))
+
+lemma is_parser_either_raw_expected [simp]:
+  "is_parser (p <|>\<r> expected_raw s) = is_parser p"
+  unfolding expected_raw_def
+  by (smt (verit, best) Inl_Inr_False either_raw_def either_raw_is_parser is_parser_def sum.case(2))
 
 subsection \<open>Additional combinators\<close>
 
@@ -113,219 +340,389 @@ abbreviation
   empty :: "('i, 'o) parser_scheme" where
   "empty \<equiv> fail ''''"
 
+subsubsection \<open>Applicative map\<close>
+
 definition
+  amap_raw :: "('i, ('a \<Rightarrow> 'b)) parser_function \<Rightarrow> ('i, 'a) parser_function \<Rightarrow> ('i, 'b) parser_function" (infixl "<*>\<r>" 58)
+where
+  "amap_raw pf px = ((\<lambda>(f, x). f x) <$>\<r> (product_raw pf px))"
+
+lemma amap_raw_is_parser [intro]:
+  assumes "is_parser pf" and "is_parser px" shows "is_parser (amap_raw pf px)"
+  unfolding amap_raw_def
+  using assms by blast
+
+lift_definition
   amap :: "('i, ('a \<Rightarrow> 'b)) parser_scheme \<Rightarrow> ('i, 'a) parser_scheme \<Rightarrow> ('i, 'b) parser_scheme" (infixl "<*>" 58)
-where
-  "amap pf px = ((\<lambda>(f, x). f x) <$> (product pf px))"
+  is amap_raw by blast
 
-definition
-  right :: "('i, 'a) parser_scheme \<Rightarrow> ('i, 'b) parser_scheme \<Rightarrow> ('i, 'b) parser_scheme" (infixl "*>" 58)
-where
-  "right p q = ((\<lambda>x.\<lambda>y. y) <$> p <*> q)"
+lemma amap_raw_is_greedy_parser [intro]:
+  assumes "greedy_parser pf" and "greedy_parser px" shows "greedy_parser (amap_raw pf px)"
+  unfolding amap_raw_def
+  using assms by blast
 
-definition
-  left :: "('i, 'a) parser_scheme \<Rightarrow> ('i, 'b) parser_scheme \<Rightarrow> ('i, 'a) parser_scheme" (infixl "<*" 58)
-where
-  "left p q = ((\<lambda>x.\<lambda>y. x) <$> p <*> q)"
+lift_definition
+  amap\<g> :: "('i, ('a \<Rightarrow> 'b)) greedy_parser_scheme \<Rightarrow> ('i, 'a) greedy_parser_scheme \<Rightarrow> ('i, 'b) greedy_parser_scheme" (infixl "<*>\<g>" 58)
+  is amap_raw by blast
 
-definition
-  entry :: "'i \<Rightarrow> ('i, 'i::show) parser_scheme" where
-  "entry s = (satisfy (\<lambda>x. x = s) <|> (expected (''entry `'' @ show s @ ''`'')))"
+lemma parser_greedy_amap_raw_is_greedy_parser [intro]:
+  assumes "is_parser pf" and "greedy_parser px" shows "greedy_parser (amap_raw pf px)"
+  unfolding amap_raw_def
+  using assms by blast
 
-definition
-  optional :: "('i, 'o) parser_scheme \<Rightarrow> ('i, 'o option) parser_scheme" where
-  "optional p = (Some <$> p <|> pure None)"
+lift_definition
+  amap\<g>\<r> :: "('i, ('a \<Rightarrow> 'b)) parser_scheme \<Rightarrow> ('i, 'a) greedy_parser_scheme \<Rightarrow> ('i, 'b) greedy_parser_scheme" (infixl "<*>\<g>\<r>" 58)
+  is amap_raw by blast
 
-function (sequential)
-  many_aux :: "('i, 'a) greedy_parser_scheme \<Rightarrow> 'a list \<Rightarrow> ('i, 'a list) parser_scheme" where
-  "many_aux p acc i =
-  (case rep_greedy p i of
-    Inl _ \<Rightarrow> Inr (i, acc)
-  | Inr (i', a) \<Rightarrow>
-    (case many_aux p (a # acc) i' of
-      Inl _ \<Rightarrow> undefined
-    | Inr (i'', a') \<Rightarrow> Inr (i'', a')))"
-by pat_completeness auto
+lemma greedy_parser_amap_raw_is_greedy_parser [intro]:
+  assumes "greedy_parser pf" and "is_parser px" shows "greedy_parser (amap_raw pf px)"
+  unfolding amap_raw_def
+  using assms by blast
 
-termination many_aux
-proof
-  show "wf (measure (\<lambda>(p, a, i). length i))" by simp
-next
-  fix p acc i x2 x y
-  assume "rep_greedy p i = Inr x2"
-    and "(x, y) = x2"
-  hence "length x < length i" using rep_greedy by fastforce
-  thus "((p, y # acc, x), p, acc, i) \<in> measure (\<lambda>(p, a, y). length y)" by auto
-qed
+lift_definition
+  amap\<g>\<l> :: "('i, ('a \<Rightarrow> 'b)) greedy_parser_scheme \<Rightarrow> ('i, 'a) parser_scheme \<Rightarrow> ('i, 'b) greedy_parser_scheme" (infixl "<*>\<g>\<l>" 58)
+  is amap_raw by blast
 
-definition
-  many :: "('i, 'a) greedy_parser_scheme \<Rightarrow> ('i, 'a list) parser_scheme" where
-  "many p = (rev <$> many_aux p [])"
-
-definition
-  many1 :: "('i, 'a) greedy_parser_scheme \<Rightarrow> ('i, 'a list) parser_scheme" where
-  "many1 p = ((#) <$> (rep_greedy p) <*> many p)"
-
-subsection \<open>Main properties\<close>
-
-lemma map_id [simp, code_unfold]:
-  "(id <$> p) = p" unfolding map_def
-  by (auto split: sum.split)
-
-lemma pure_f_amap [simp, code_unfold]:
-  "(pure f <*> p) = (f <$> p)"
-  unfolding amap_def map_def pure_def product_def
+lemma pure_raw_f_amap [simp, code_unfold]:
+  "(pure_raw f <*>\<r> p) = (f <$>\<r> p)"
+  unfolding amap_raw_def map_raw_def pure_raw_def product_raw_def bind_raw_def
   by (auto split: sum.split)
 
 lemma applicative_identity [simp, code_unfold]:
-  "(pure id <*> p) = p"
-  by simp
+  "(pure_raw id <*>\<r> p) = p"
+  unfolding pure_raw_def amap_raw_def map_raw_def product_raw_def bind_raw_def
+  by (auto split: sum.split)
 
 lemma applicative_homomorphism [simp, code_unfold]:
-  "(pure f <*> pure x) = pure (f x)"
-  unfolding map_def pure_def amap_def product_def
+  "(pure_raw f <*>\<r> pure_raw x) = pure_raw (f x)"
+  unfolding map_raw_def pure_raw_def amap_raw_def product_raw_def bind_raw_def
   by (auto split: sum.split)
 
 lemma applicative_interchange:
-  "(u <*> pure x) = (pure (\<lambda>f. f x) <*> u)"
-  unfolding product_def pure_def amap_def map_def
+  "(u <*>\<r> pure_raw x) = (pure_raw (\<lambda>f. f x) <*>\<r> u)"
+  unfolding product_raw_def pure_raw_def amap_raw_def map_raw_def bind_raw_def
   by (auto split: sum.split)
 
 lemma applicative_composition [simp]:
-  "(((pure (\<circ>) <*> u) <*> v) <*> w) = (u <*> (v <*> w))"
-  unfolding pure_def map_def amap_def product_def
+  "(((pure_raw (\<circ>) <*>\<r> u) <*>\<r> v) <*>\<r> w) = (u <*>\<r> (v <*>\<r> w))"
+  unfolding pure_raw_def map_raw_def amap_raw_def product_raw_def bind_raw_def
   by (auto split: sum.split)
 
-lemma alternative_identity_left [simp, code_unfold]:
-  "(empty <|> u) = u"
-  unfolding empty_def fail_def either_def
-  by simp
+subsubsection \<open>Right\<close>
+definition
+  right_raw :: "('i, 'a) parser_function \<Rightarrow> ('i, 'b) parser_function \<Rightarrow> ('i, 'b) parser_function" (infixl "*>\<r>" 58)
+where
+  "right_raw p q = ((\<lambda>x.\<lambda>y. y) <$>\<r> p <*>\<r> q)"
 
-(* NOTE: Broken due to migration to sum type *)
-(* lemma alternative_identity_right [simp, code_unfold]:
- *   "(p <|> empty) = p"
- *   unfolding either_def empty_def fail_def
- *   by (auto split: sum.split) *)
+lemma right_raw_is_parser [intro]:
+  assumes "is_parser p" and "is_parser q" shows "is_parser (right_raw p q)"
+  unfolding right_raw_def
+  using assms by blast
 
-lemma alternative_associativity:
-  "(u <|> (v <|> w)) = ((u <|> v) <|> w)"
-  unfolding either_def
-  by (auto split: sum.split)
+lift_definition
+  right :: "('i, 'a) parser_scheme \<Rightarrow> ('i, 'b) parser_scheme \<Rightarrow> ('i, 'b) parser_scheme" (infixl "*>" 58)
+  is right_raw by blast
 
-subsubsection \<open>Consumption analysis\<close>
+lemma right_raw_is_greedy_parser [intro]:
+  assumes "greedy_parser p" and "greedy_parser q" shows "greedy_parser (right_raw p q)"
+  unfolding right_raw_def
+  using assms by blast
 
-text \<open>We've defined two type of predicates that check if parser not producs new input both strict and non-strict.\<close>
+lift_definition
+  right\<g> :: "('i, 'a) greedy_parser_scheme \<Rightarrow> ('i, 'b) greedy_parser_scheme \<Rightarrow> ('i, 'b) greedy_parser_scheme" (infixl "*>\<g>" 58)
+  is right_raw by blast
 
-lemma fail_is_parser [intro]:
-  "is_parser (fail s)"
-  by (simp add: is_parser_def fail_def)
+lemma parser_greedy_right_raw_is_greedy_parser [intro]:
+  assumes "is_parser p" and "greedy_parser q" shows "greedy_parser (right_raw p q)"
+  unfolding right_raw_def
+  using assms by blast
 
-lemma pure_is_parser [intro]:
-  "is_parser (pure x)"
-  by (simp add: is_parser_def pure_def)
+lift_definition
+  right\<g>\<r> :: "('i, 'a) parser_scheme \<Rightarrow> ('i, 'b) greedy_parser_scheme \<Rightarrow> ('i, 'b) greedy_parser_scheme" (infixl "*>\<g>\<r>" 58)
+  is right_raw by blast
 
-lemma satisfy_is_greedy_parser [intro]:
-  "greedy_parser (satisfy P)"
-  by (simp add: greedy_parser_def list.case_eq_if satisfy_def expected_def)
+lemma greedy_parser_right_raw_is_greedy_parser [intro]:
+  assumes "greedy_parser p" and "is_parser q" shows "greedy_parser (right_raw p q)"
+  unfolding right_raw_def
+  using assms by blast
 
-lemma bind_is_greedy_parser [intro]:
-  assumes "greedy_parser p" and "\<And>x. greedy_parser (f x)" shows "greedy_parser (bind p f)"
-  unfolding greedy_parser_def
-  by (smt (verit) Inl_Inr_False ParserCombinators.bind_def assms greedy_parserE order_less_trans prod.split_sel split_beta sum.case_eq_if sum.collapse(2) sum.disc(2))
+lift_definition
+  right\<g>\<l> :: "('i, 'a') greedy_parser_scheme \<Rightarrow> ('i, 'b) parser_scheme \<Rightarrow> ('i, 'b) greedy_parser_scheme" (infixl "*>\<g>\<l>" 58)
+  is right_raw by blast
 
-lemma map_is_greedy_parser [intro]:
-  assumes "greedy_parser p" shows "greedy_parser (map f p)"
-  using assms unfolding is_parser_def greedy_parser_def map_def
-  by (smt (verit, best) Inl_Inr_False Inr_inject fstI old.prod.exhaust old.sum.exhaust split_beta sum.case(1) sum.case(2))
+subsubsection \<open>Left\<close>
+definition
+  left_raw :: "('i, 'a) parser_function \<Rightarrow> ('i, 'b) parser_function \<Rightarrow> ('i, 'a) parser_function" (infixl "<*\<r>" 58)
+where
+  "left_raw p q = ((\<lambda>x.\<lambda>y. x) <$>\<r> p <*>\<r> q)"
 
-lemma product_is_greedy_parser [intro]:
-  assumes "greedy_parser p" and "greedy_parser q" shows "greedy_parser (product p q)"
-  unfolding product_def greedy_parser_def
-  by (smt (verit, best) Inl_Inr_False assms dual_order.strict_trans2 fstI greedy_parserE less_imp_le_nat prod.collapse split_beta sum.case_eq_if sum.collapse(2) sum.sel(2))
+lemma left_raw_is_parser [intro]:
+  assumes "is_parser p" and "is_parser q" shows "is_parser (left_raw p q)"
+  unfolding left_raw_def
+  using assms by blast
 
-lemma either_greedy_parsers:
-  assumes "greedy_parser (either p q)" shows "greedy_parser p \<or> greedy_parser q"
-  unfolding either_def greedy_parser_def
-  by (metis assms either_def greedy_parser_def sum.case(2))
+lift_definition
+  left :: "('i, 'a) parser_scheme \<Rightarrow> ('i, 'b) parser_scheme \<Rightarrow> ('i, 'a) parser_scheme" (infixl "<*" 58)
+  is left_raw by blast
 
-lemma either_is_greedy_parser [intro]:
-  assumes "greedy_parser p" and "greedy_parser q" shows "greedy_parser (either p q)"
-  unfolding either_def
-  by (metis (mono_tags, lifting) assms greedy_parser_def sum.case_eq_if sum.collapse(2))
+lemma left_raw_is_greedy_parser [intro]:
+  assumes "greedy_parser p" and "greedy_parser q" shows "greedy_parser (left_raw p q)"
+  unfolding left_raw_def
+  using assms by blast
 
-lemma either_parsers:
-  assumes "is_parser (either p q)" shows "is_parser p \<or> is_parser q"
-  unfolding is_parser_def either_def
-  by (metis assms either_def is_parser_def sum.case(2))
+lift_definition
+  left\<g> :: "('i, 'a) greedy_parser_scheme \<Rightarrow> ('i, 'b) greedy_parser_scheme \<Rightarrow> ('i, 'a) greedy_parser_scheme" (infixl "<*\<g>" 58)
+  is left_raw by blast
 
-lemma either_is_parser [intro]:
-  assumes "is_parser p" and "is_parser q" shows "is_parser (either p q)"
-  unfolding either_def
-  by (smt (verit) assms is_parser_def sum.case_eq_if sum.disc(2) sum.expand sum.sel(2))
+lemma parser_greedy_left_raw_is_greedy_parser [intro]:
+  assumes "is_parser p" and "greedy_parser q" shows "greedy_parser (left_raw p q)"
+  unfolding left_raw_def
+  using assms by blast
 
-lemma greedy_parser_either_fail [simp]:
-  "greedy_parser (p <|> fail s) = greedy_parser p"
-  by (metis (mono_tags, lifting) Inl_Inr_False either_def either_is_greedy_parser fail_def greedy_parser_def old.sum.simps(6))
+lift_definition
+  left\<g>\<r> :: "('i, 'a) parser_scheme \<Rightarrow> ('i, 'b) greedy_parser_scheme \<Rightarrow> ('i, 'a) greedy_parser_scheme" (infixl "<*\<g>\<r>" 58)
+  is left_raw by blast
 
-lemma greedy_parser_either_expected [simp]:
-  "greedy_parser (p <|> expected s) = greedy_parser p"
-  unfolding expected_def
-  by (smt (verit, best) Inl_Inr_False either_def either_is_greedy_parser greedy_parser_def sum.case(2))
+lemma greedy_parser_left_raw_is_greedy_parser [intro]:
+  assumes "greedy_parser p" and "is_parser q" shows "greedy_parser (left_raw p q)"
+  unfolding left_raw_def
+  using assms by blast
 
-lemma amap_is_greedy_parser [intro]:
-  assumes "greedy_parser pf" and "greedy_parser px" shows "greedy_parser (amap pf px)"
-  by (simp add: amap_def assms(1) assms(2) map_is_greedy_parser product_is_greedy_parser)
+lift_definition
+  left\<g>\<l> :: "('i, 'a) greedy_parser_scheme \<Rightarrow> ('i, 'b) parser_scheme \<Rightarrow> ('i, 'a) greedy_parser_scheme" (infixl "<*\<g>\<l>" 58)
+  is left_raw by blast
 
-lemma right_is_greedy_parser [intro]:
-  assumes "greedy_parser p" and "greedy_parser q" shows "greedy_parser (right p q)"
-  by (simp add: amap_is_greedy_parser assms map_is_greedy_parser right_def)
+subsubsection \<open>Entry\<close>
+definition
+  entry_raw :: "'i \<Rightarrow> ('i, 'i::show) parser_function" where
+  "entry_raw s = (satisfy_raw (\<lambda>x. x = s) <|>\<r> (expected_raw (''entry `'' @ show s @ ''`'')))"
 
-lemma left_is_greedy_parser [intro]:
-  assumes "greedy_parser p" and "greedy_parser q" shows "greedy_parser (left p q)"
-  by (simp add: amap_is_greedy_parser assms map_is_greedy_parser left_def)
-
-lemma entry_is_greedy_parser[intro]:
-  "greedy_parser (entry c)"
-  unfolding entry_def
+lemma entry_is_greedy_parser [intro]:
+  "greedy_parser (entry_raw c)"
+  unfolding entry_raw_def
   by (simp add: satisfy_is_greedy_parser)
 
-lemma optional_is_parser[intro]:
-  assumes "is_parser p" shows "is_parser (optional p)"
-  unfolding optional_def
-  by (smt (z3) ParserCombinators.map_def assms case_prod_unfold either_def eq_fst_iff is_parserE is_parserI old.sum.simps(5) pure_is_parser sum.case_eq_if sum.collapse(2) sum.sel(2))
+lift_definition
+  entry :: "'i \<Rightarrow> ('i, 'i::show) parser_scheme"
+  is entry_raw by (simp add: entry_is_greedy_parser greedy_parser_implies_is_parser)
 
-subsection \<open>Greedy lifted definitions\<close>
+lift_definition
+  entry\<g> :: "'i \<Rightarrow> ('i, 'i::show) greedy_parser_scheme"
+  is entry_raw by blast
 
-text \<open>In order to construct parsers that repeat many times we introduce convention for lifted defintions of greedy parsers - postfix `G`.\<close>
+subsubsection \<open>Exactly\<close>
 
-lift_definition satisfyG :: "('i \<Rightarrow> bool) \<Rightarrow> ('i::show, 'i) greedy_parser_scheme"
-  is satisfy by blast
+definition
+  exactly_raw ::  "'i list \<Rightarrow> ('i, 'i::show list) parser_function" where
+  "exactly_raw s i =
+  (if prefix s i \<and> length s > 0
+  then Inr (drop (length s) i, take (length s) i)
+  else expected_raw (''exactly \"'' @ show s @ ''\"'') i)"
 
-lift_definition bindG :: "('i, 'a) greedy_parser_scheme \<Rightarrow> ('a \<Rightarrow> ('i, 'b) greedy_parser_scheme) \<Rightarrow> ('i, 'b) greedy_parser_scheme"
-  is bind by blast
+lemma exactly_raw_is_parser [intro]:
+  "is_parser (exactly_raw s)"
+  unfolding is_parser_def exactly_raw_def expected_raw_def
+  by simp
 
-adhoc_overloading
-  Monad_Syntax.bind bindG
+lemma exactly_raw_is_greedy_parser [intro]:
+  "greedy_parser (exactly_raw s)"
+  unfolding greedy_parser_def exactly_raw_def expected_raw_def
+  by (metis Inl_Inr_False Inr_inject Pair_inject diff_less length_drop length_greater_0_conv prefix_bot.extremum_unique)
 
-lift_definition mapG :: "('a \<Rightarrow> 'b) \<Rightarrow> ('i, 'a) greedy_parser_scheme \<Rightarrow> ('i, 'b) greedy_parser_scheme" (infixl "<$>G" 58)
-  is map by blast
+lift_definition
+  exactly :: "'i list \<Rightarrow> ('i, 'i::show list) parser_scheme"
+  is exactly_raw by blast
 
-lift_definition productG :: "('i, 'a) greedy_parser_scheme \<Rightarrow> ('i, 'b) greedy_parser_scheme \<Rightarrow> ('i, 'a \<times> 'b) greedy_parser_scheme"
-  is product by blast
+lift_definition
+  exactly\<g> :: "'i list \<Rightarrow> ('i, 'i::show list) greedy_parser_scheme"
+  is exactly_raw by blast
 
-lift_definition eitherG :: "('i, 'a) greedy_parser_scheme \<Rightarrow> ('i, 'a) greedy_parser_scheme \<Rightarrow> ('i, 'a) greedy_parser_scheme" (infixl "<|>G" 57)
-  is either by blast
+subsubsection \<open>Optional\<close>
+definition
+  optional_raw :: "('i, 'o) parser_function \<Rightarrow> ('i, 'o option) parser_function" where
+  "optional_raw p = (Some <$>\<r> p <|>\<r> pure_raw None)"
 
-lift_definition amapG :: "('i, ('a \<Rightarrow> 'b)) greedy_parser_scheme \<Rightarrow> ('i, 'a) greedy_parser_scheme \<Rightarrow> ('i, 'b) greedy_parser_scheme" (infixl "<*>G" 58)
-  is amap by blast
+lemma optional_raw_is_parser [intro]:
+  assumes "is_parser p" shows "is_parser (optional_raw p)"
+  unfolding optional_raw_def
+  by (simp add: assms either_raw_is_parser map_raw_is_parser pure_raw_is_parser)
 
-lift_definition rightG :: "('i, 'a) greedy_parser_scheme \<Rightarrow> ('i, 'b) greedy_parser_scheme \<Rightarrow> ('i, 'b) greedy_parser_scheme" (infixl "*>G" 58)
-  is right by blast
+lift_definition
+  optional :: "('i, 'o) parser_scheme \<Rightarrow> ('i, 'o option) parser_scheme"
+  is optional_raw by blast
 
-lift_definition leftG :: "('i, 'a) greedy_parser_scheme \<Rightarrow> ('i, 'b) greedy_parser_scheme \<Rightarrow> ('i, 'a) greedy_parser_scheme" (infixl "<*G" 58)
-  is left by blast
+subsubsection \<open>Repeated\<close>
+fun
+  repeated_raw :: "nat \<Rightarrow> ('i, 'o) parser_function \<Rightarrow> ('i, 'o list) parser_function" where
+  "repeated_raw 0 p = pure_raw []" |
+  "repeated_raw (Suc n) p = ((#) <$>\<r> p <*>\<r> repeated_raw n p)"
 
-lift_definition entryG :: "'i \<Rightarrow> ('i, 'i::show) greedy_parser_scheme"
-  is entry by blast
+lemma repeated_raw_is_parser [intro]:
+  assumes "is_parser p" shows "is_parser (repeated_raw n p)"
+proof (induction n)
+  case 0
+  thus ?case
+    by (simp add: pure_raw_is_parser)
+next
+  case (Suc n)
+  thus ?case
+  proof
+    assume "(\<And>i r v. repeated_raw n p i = Inr (r, v) \<Longrightarrow> length r \<le> length i)"
+    show "is_parser (repeated_raw (Suc n) p)"
+      using repeated_raw.simps
+      by (simp add: Suc amap_raw_is_parser assms map_raw_is_parser)
+  qed
+qed
+
+lift_definition
+  repeated :: "nat \<Rightarrow> ('i, 'o) parser_scheme \<Rightarrow> ('i, 'o list) parser_scheme"
+  is repeated_raw by blast
+
+lemma repeated_raw_is_greedy [intro]:
+  assumes "greedy_parser p" shows "greedy_parser (repeated_raw (Suc n) p)"
+proof (induction n)
+  case 0
+  thus ?case
+    unfolding repeated_raw.simps
+    using assms
+    by blast
+next
+  case (Suc n)
+  thus ?case unfolding repeated_raw.simps(2)
+    by (simp add: amap_raw_is_greedy_parser assms map_raw_is_greedy_parser)
+qed
+
+text \<open>Please be aware that this function just adds 1 to the number of repetitions!\<close>
+lift_definition
+  repeated\<g> :: "nat \<Rightarrow> ('i, 'o) greedy_parser_scheme \<Rightarrow> ('i, 'o list) greedy_parser_scheme"
+  is "(\<lambda>n. repeated_raw (Suc n))" using repeated_raw_is_greedy by auto
+
+lemma repeated_raw_pure_eq_pure_raw_replicate [simp, code_unfold]:
+  "repeated_raw n (pure_raw x) = pure_raw (replicate n x)"
+proof (induction n)
+  case 0
+  thus ?case by simp
+next
+  case (Suc n)
+  moreover have "(amap_raw (map_raw (#) (pure_raw x)) (pure_raw (replicate n x))) = pure_raw (replicate (Suc n) x)"
+    by (metis applicative_homomorphism pure_raw_f_amap replicate_Suc)
+  ultimately show ?case unfolding repeated_raw.simps by simp
+qed
+
+subsubsection \<open>Many\<close>
+
+function
+  many_raw :: "('i, 'o) greedy_parser_scheme \<Rightarrow> ('i, 'o list) parser_function" where
+  "many_raw p i =
+  (case run_greedy p i of
+    Inl _ \<Rightarrow> Inr (i, [])
+  | Inr (r, v) \<Rightarrow>
+    (case many_raw p r of
+      Inl _ \<Rightarrow> Inr (r, [v])
+    | Inr (r', v') \<Rightarrow> Inr (r', (v # v'))))"
+by auto
+
+termination
+  using run_greedy
+  by (relation \<open>measure (\<lambda>(_, i). length i)\<close>) fastforce+
+
+lemma many_raw_is_parser [intro]:
+  "is_parser (many_raw p)" unfolding is_parser_def
+proof
+  show "\<forall>r v. many_raw p i = Inr (r, v) \<longrightarrow> length r \<le> length i" for i
+  proof (induct rule: many_raw.induct)
+    case (1 xs) thus ?case
+      using run_greedy
+      by (subst many_raw.simps)
+         (fastforce split: sum.splits simp del: many_raw.simps)
+  qed
+qed
+
+lift_definition
+  many :: "('i, 'o) greedy_parser_scheme \<Rightarrow> ('i, 'o list) parser_scheme"
+  is many_raw by blast
+
+subsubsection \<open>Many1\<close>
+definition
+  many1_raw :: "('i, 'o) greedy_parser_scheme \<Rightarrow> ('i, 'o list) parser_function" where
+  "many1_raw p = ((#) <$>\<r> run_greedy p <*>\<r> many_raw p)"
+
+lemma many1_raw_is_greedy_parser [intro]:
+  "greedy_parser (many1_raw p)"
+  unfolding many1_raw_def
+proof -
+  have "greedy_parser (map_raw (#) (run_greedy p))" using run_greedy by auto
+  moreover have "is_parser (many_raw p)" by auto
+  ultimately show "greedy_parser (amap_raw (map_raw (#) (run_greedy p)) (many_raw p))" by auto
+qed
+
+lemma many1_raw_is_parser [intro]:
+  "is_parser (many1_raw p)"
+  by (simp add: greedy_parser_implies_is_parser many1_raw_is_greedy_parser)
+
+lift_definition
+  many1 :: "('i, 'o) greedy_parser_scheme \<Rightarrow> ('i, 'o list) parser_scheme"
+  is many1_raw by blast
+
+lift_definition
+  many1\<g> :: "('i, 'o) greedy_parser_scheme \<Rightarrow> ('i, 'o list) greedy_parser_scheme"
+  is many1_raw by blast
+
+subsubsection \<open>Separated by, at least one\<close>
+definition
+  sep_by1 :: "('i, 'sep) greedy_parser_scheme \<Rightarrow> ('i, 'o) greedy_parser_scheme \<Rightarrow> ('i, 'o list) greedy_parser_scheme" where
+  "sep_by1 sep p = ((#) <$>\<g> p <*>\<g>\<l> (many (sep *>\<g> p)))"
+
+subsubsection \<open>Separated by\<close>
+definition
+  sep_by :: "('i, 'sep) greedy_parser_scheme \<Rightarrow> ('i, 'o) greedy_parser_scheme \<Rightarrow> ('i, 'o list) parser_scheme" where
+  "sep_by sep p = (sep_by1 sep p <|>\<p>\<r> pure [])"
+
+subsubsection \<open>Take while\<close>
+definition
+  take_while :: "('i \<Rightarrow> bool) \<Rightarrow> ('i, 'i::show list) parser_scheme" where
+  "take_while p = many (satisfy\<g> p)"
+
+subsubsection \<open>Drop while\<close>
+definition
+  drop_while :: "('i::show \<Rightarrow> bool) \<Rightarrow> ('i, unit) parser_scheme" where
+  "drop_while p = ((\<lambda>_. ()) <$> many (satisfy\<g> p))"
+
+subsection \<open>Common parsers\<close>
+
+subsubsection \<open>Ascii white space\<close>
+text \<open>Removes all characters that belong to ASCII white space characters: ' ', '\t', '\r', '\n', '\f', '\v'\<close>
+definition
+  ascii_space_chars :: "char list" where
+  "ascii_space_chars = List.map char_of [0x20::nat, 0x9, 0xd, 0xa, 0xc, 0xb]"
+
+definition
+  ascii_spaces :: "(char, unit) parser_scheme" where
+  "ascii_spaces = ((\<lambda>_. Unity) <$> many (satisfy\<g> (\<lambda>c. c \<in> (set ascii_space_chars))))"
+
+definition
+  ascii_spaces\<g> :: "(char, unit) greedy_parser_scheme" where
+  "ascii_spaces\<g> = ((\<lambda>_. Unity) <$>\<g> many1\<g> (satisfy\<g> (\<lambda>c. c \<in> (set ascii_space_chars))))"
+
+subsubsection \<open>Number\<close>
+definition
+  alphabet :: string where
+  "alphabet = ''0123456789ABCDEF''"
+
+definition
+  nat_of_char :: "char \<Rightarrow> nat" where
+  "nat_of_char c = of_char c - (of_char CHR ''0'')"
+
+definition
+  decimal_digit :: "(char, nat) greedy_parser_scheme" where
+  "decimal_digit = (nat_of_char <$>\<g> (satisfy\<g> (\<lambda>c. c \<in> set (take 10 alphabet))))"
+
+definition
+  nat_of_decimal_digits :: "nat list \<Rightarrow> nat" where
+  "nat_of_decimal_digits = foldl (\<lambda>a n. a * 10 + n) 0"
+
+definition
+  decimal :: "(char, nat) greedy_parser_scheme" where
+  "decimal = (nat_of_decimal_digits <$>\<g> many1\<g> decimal_digit)"
 
 end
